Induction.v
@@ -475,6 +475,7 @@ Qed.
 Theorem S_nbeq_0 : forall n:nat,
   beq_nat (S n) 0 = false.
 Proof.
+  
   (* FILL IN HERE *) Admitted.
 
 Theorem mult_1_l : forall n:nat, 1 * n = n.
